aspirations of proving correctness

ArrowPoly/ArrayExtra.lean
@@ -1,7 +1,20 @@
-theorem not_or (p q) : ¬ (p ∨ q) ↔ ¬ p ∧ ¬ q :=
-⟨fun H => ⟨mt Or.inl H, mt Or.inr H⟩, fun ⟨hp, hq⟩ pq => pq.elim hp hq⟩
+import ArrowPoly.NatExtra
+import ArrowPoly.ListExtra
+import ArrowPoly.LogicExtra
 
-def Array.dropZeros (a : Array Int) : Array Int :=
+theorem Array.back_eq_of_back?_eq [Inhabited α] {a : Array α} (h : a.back? = some x) :
+  a.back = x :=
+by
+  simp [back?, get?, get] at h
+  split at h
+  · rename_i h'
+    cases h
+    simp [back, get!, getD, h', get]
+  · cases h
+
+
+/-- Pop off trailing zeros -/
+def Array.popZeros (a : Array Int) : Array Int :=
   if h : a.isEmpty ∨ a.back ≠ 0 then
     a
   else
@@ -9,22 +22,8 @@ def Array.dropZeros (a : Array Int) : Array Int :=
       simp [not_or, isEmpty] at h
       show _ ≤ _
       simp [h.1, Nat.sub_succ, Nat.succ_pred]
-    dropZeros a.pop
+    popZeros a.pop
 termination_by _ => a.size
-
-/-
-def Array.dropZeros (a : Array Int) : Array Int :=
-  let rec aux : Nat → Array Int → Array Int
-          | 0, _ => a
-          | n+1, a => if a.back ≠ 0 then a else aux n a.pop
-  aux a.size a
--/
-
-@[simp]
-theorem not_not (p : Prop) : ¬¬p ↔ p := by
-  cases Classical.em p with
-  | inl h => simp [h]
-  | inr h => simp [h]
 
 theorem Array.back?_eq_of_size_eq_zero (a : Array Int) (h : a.size = 0) : a.back? = none := by
   simp [back?, h]
@@ -34,70 +33,34 @@ theorem Array.back?_eq_of_size_eq_zero (a : Array Int) (h : a.size = 0) : a.back
   | nil => rfl
   | cons x xs => cases h
 
-theorem Array.back?_dropZeros (a : Array Int) : a.dropZeros.back? ≠ some 0 := by
-  rw [dropZeros]
+theorem Array.back?_popZeros (a : Array Int) : a.popZeros.back? ≠ some 0 := by
+  rw [popZeros]
   simp []
   split
-  rename_i h
-  simp [isEmpty] at h
-  cases h with
-  | inl h => simp [Array.back?_eq_of_size_eq_zero _ h]
-  | inr h =>
-    simp [back?, get?]
-    split
-    rename_i h'
-    simp
-    simp [back, get!, getD, h'] at h
-    exact h
-    simp
-  rename_i h
-  have : size a - 1 < size a := by
-    simp [not_or, isEmpty] at h
-    have : ∃ n, size a = n := ⟨_, rfl⟩
-    cases this with
-    | intro n h' =>
-      simp [h']
-      simp [h'] at h
-      cases n
-      exact False.elim (h.1 rfl)
-      show _ ≤ _
-      apply Nat.le_refl
-  apply back?_dropZeros
+  · rename_i h
+    simp [isEmpty] at h
+    cases h with
+    | inl h => simp [Array.back?_eq_of_size_eq_zero _ h]
+    | inr h => exact Array.back_eq_of_back?_eq.mt h
+  · rename_i h
+    have : size a - 1 < size a := by
+      simp [not_or, isEmpty] at h
+      apply Nat.pred_le_self_of_ne_zero _ h.1
+    apply back?_popZeros
 termination_by _ => a.size
-
-theorem List.concat_cons (x : α) (xs : List α) (y : α) :
-  (x :: xs).concat y = x :: xs.concat y := rfl
-
-@[simp]
-theorem List.get_concat (x y : α) (xs : List α) (i : Fin (xs.concat y).length) :
-  ((x :: xs).concat y).get i.succ = (xs.concat y).get i := rfl
-
-@[simp]
-theorem List.get_concat_last (xs : List α) (y : α) (h : xs.length < (xs.concat y).length) :
-  (xs.concat y).get ⟨xs.length, h⟩ = y :=
-by
-  induction xs with
-  | nil => rfl
-  | cons x xs ih =>
-    have : length xs < length (concat xs y) := by
-      simp
-      apply Nat.lt_succ_self
-    have := List.get_concat x y xs ⟨xs.length, this⟩
-    rw [ih] at this
-    exact this
 
 @[simp]
 theorem Array.back?_push (a : Array α) [Inhabited α] (x : α) : (a.push x).back? = some x := by
   simp [back?, push, get?, get]
   split
-  rename_i h
-  simp [Nat.add_sub_self_right]
-  
-  rename_i h
-  apply h
-  simp [Nat.add_sub_self_right]
-  apply Nat.lt_succ_self
+  · rename_i h
+    simp [Nat.add_sub_self_right]
+  · rename_i h
+    apply h
+    simp [Nat.add_sub_self_right]
+    apply Nat.lt_succ_self
 
+/-- Get the element if the index is in range, else return `default`. -/
 @[inline] def Array.get!? (a : Array α) (i : Nat) (default : α) : α :=
 if h : i < a.size then a.get ⟨i, h⟩ else default
 
@@ -109,6 +72,7 @@ if h : i < a.size then a.get ⟨i, h⟩ else default
     cs
 termination_by _ => max as.size bs.size - i
 
+/-- Like `Array.zipWith`, but extend the arrays with `default` so they match lengths. -/
 @[inline] def Array.zipWith' [Inhabited α] [Inhabited β]
   (as : Array α) (bs : Array β) (f : α → β → γ) : Array γ :=
   zipWith'Aux f as bs 0 #[]
@@ -125,28 +89,29 @@ termination_by _ => max as.size bs.size - i
 @[inline] def Array.lexicographic [Ord α] [Inhabited α] : Ord (Array α) where
   compare as bs := Array.lexicographicAux as bs 0
 
-inductive Merge α
+inductive Merge (α : Type _)
 | left (x : α)
 | right (x : α)
 | both (x y : α)
+deriving Repr
 
 section merge
-variable (f : α → β) [Ord β] (g : Array γ → Merge α → Array γ) 
+variable (f : α → β) [Ord β] (g : γ → Merge α → γ) 
 
-def Array.mergeByAuxLeft (as : Array α) (i : Nat) (cs : Array γ) : Array γ :=
+def Array.mergeByAuxLeft (as : Array α) (i : Nat) (cs : γ) : γ :=
   if h : i < as.size then
       mergeByAuxLeft as (i+1) <| g cs (.left <| as.get ⟨i, h⟩)
   else cs
 termination_by _ => as.size - i
 
-def Array.mergeByAuxRight (bs : Array α) (j : Nat) (cs : Array γ) : Array γ :=
+def Array.mergeByAuxRight (bs : Array α) (j : Nat) (cs : γ) : γ :=
   if h : j < bs.size then
       mergeByAuxRight bs (j+1) <| g cs (.right <| bs.get ⟨j, h⟩)
   else cs
 termination_by _ => bs.size - j
 
 @[specialize]
-def Array.mergeByAux (as bs : Array α) (i j : Nat) (cs : Array γ) : Array γ :=
+def Array.mergeByAux (as bs : Array α) (i j : Nat) (cs : γ) : γ :=
   if h : i < as.size ∧ j < bs.size then
     match compare (f <| as.get ⟨i, h.1⟩) (f <| bs.get ⟨j, h.2⟩) with
     | .lt =>
@@ -175,9 +140,164 @@ def Array.mergeByAux (as bs : Array α) (i j : Nat) (cs : Array γ) : Array γ :
   else cs
 termination_by _ => (as.size - i) + (bs.size - j)
 
+/-- Assuming the arrays are sorted with respect to `f`, merge them fold the result
+using `g`.  -/
 @[inline]
-def Array.mergeBy (f : α → β) [Ord β]
-  (g : Array γ → Merge α → Array γ) (as bs : Array α) : Array γ :=
-  .mergeByAux f g as bs 0 0 #[]
+def Array.mergeBy (init : γ) (as bs : Array α) : γ :=
+  Array.mergeByAux f g as bs 0 0 init
+
+--#eval Array.mergeBy id Array.push #[] #[1,2,4] #[1,3]
 
 end merge
+
+@[simp] theorem Array.empty_size : (#[] : Array α).size = 0 := rfl
+
+theorem Array.get_push (as : Array α) (a : α) (i : Nat) (h : i < as.size) :
+  (as.push a).get ⟨i, by { simp; apply Nat.lt.step h }⟩ = as.get ⟨i, h⟩ :=
+by
+  simp [get, push]
+  cases as with
+  | mk lst => apply List.get_concat
+
+@[simp]
+theorem Array.get_push_last (as : Array α) (a : α) :
+  (as.push a).get ⟨as.size, by { simp; apply Nat.lt_succ_self }⟩ = a :=
+by simp [get, push]
+
+/-
+@[simp] theorem Array.size_map (as : Array α) (f : α → β) :
+  (as.map f).size = as.size :=
+by
+  cases as with | mk xs =>
+  simp [size, map, Id.run, mapM, foldlM, push, get, mkEmpty]
+  induction xs using List.concat_ind with
+  | nil => rfl
+  | concat xs x ih =>
+    simp
+    rw [foldlM.loop]
+    simp [Nat.zero_lt_succ]
+    simp [← Nat.succ_eq_add_one]
+-/
+
+--theorem Array.map_get 
+
+section strict_increasing
+variable [LT α]
+
+def Array.allTrue (as : Array α) (f : α → Prop) : Prop :=
+∀ (i : Fin as.size), f (as.get i)
+
+def Array.strictIncreasing (as : Array α) : Prop :=
+∀ (i j : Fin as.size), i < j → as.get i < as.get j
+
+theorem Array.strictIncreasing_empty : (#[] : Array α).strictIncreasing :=
+by
+  intros i j hij
+  cases i
+  rename_i h
+  exact (Nat.not_lt_zero _ h).elim
+
+theorem Array.strictIncreasing_push (as : Array α) (a : α) :
+  (as.push a).strictIncreasing ↔ as.strictIncreasing ∧ as.allTrue (· < a) where
+  mp := by
+    intro h
+    apply And.intro
+    · intros i j hij
+      specialize h ⟨i, _⟩ ⟨j, _⟩ hij
+      · simp [Array.get_push as a j j.isLt] at h
+        rw [Array.get_push as a i _] at h
+        exact h
+      · simp [Nat.lt.step j.isLt]
+    · intro i
+      specialize h ⟨i, _⟩ ⟨as.size, _⟩ i.isLt
+      · simp [Array.get_push as a i i.isLt, Array.get_push_last] at h
+        exact h
+      · simp [Nat.lt.step i.isLt]
+      · simp [Nat.lt_succ_self]
+  mpr := by
+    intros h i j hij
+    cases h with | intro h h' =>
+      cases Classical.em (i < as.size) with
+      | inl h'' =>
+        rw [Array.get_push as a i h'']
+        cases Classical.em (j < as.size) with
+        | inl h''' =>
+          rw [Array.get_push as a j h''']
+          exact h _ _ hij
+        | inr h''' =>
+          cases j with | mk j hj =>
+          simp at hj
+          cases Nat.eq_of_not_lt_and_lt_succ h''' hj
+          simp
+          apply h'
+      | inr h'' =>
+        cases i with | mk i hi =>
+        simp at hi
+        cases Nat.eq_of_not_lt_and_lt_succ h'' hi
+        simp at *
+        cases j with | mk j hj =>
+        simp at hij
+        cases Classical.em (j < as.size) with
+        | inl h''' =>
+          have hij' := Nat.lt_trans hij h'''
+          simp at hij'
+        | inr h''' =>
+          simp at hj
+          cases Nat.eq_of_not_lt_and_lt_succ h''' hj
+          have : List.length as.data < List.length as.data := hij
+          simp at this
+
+
+
+--theorem Array.strictIncreasing_pop (a : Array α) (h : a.strictIncreasing) :
+--  a.pop.strictIncreasing := by
+
+--theorem Array.get_pop (as : Array α) (i : Nat) (h : i < as.)
+
+theorem Array.push_pop (as : Array α) (h : as.size - 1 < as.size) :
+  as.pop.push (as.get ⟨as.size - 1, h⟩) = as :=
+by
+  cases as with | mk xs =>
+  simp [push, pop, get, size]
+  induction xs with
+  | nil => simp at h
+  | cons x xs ih =>
+    cases xs with
+    | nil => rfl
+    | cons x' xs =>
+      simp [List.dropLast, List.concat, List.get]
+      simp [Nat.pred_succ] at ih
+      have : ∀ (k : Nat), k.succ - 1 = k := λ k => rfl
+      simp [size, this] at h
+      apply ih h
+
+section ind
+
+theorem Array.eq_empty_of_isEmpty {as : Array α} (h : as.isEmpty) : as = #[] :=
+by
+  cases as with | mk lst =>
+  cases lst with
+  | nil => rfl
+  | cons x xs => simp [isEmpty] at h
+
+theorem Array.ind_push {motive : Array α → Prop}
+  (empty : motive #[])
+  (push : (as : Array α) → (a : α) → motive as → motive (as.push a))
+  (as : Array α) : motive as :=
+if h : as.isEmpty then
+  by
+    have h := Array.eq_empty_of_isEmpty h
+    cases h
+    exact empty
+else
+  by
+    simp [isEmpty] at h
+    have : size as - 1 < size as := Nat.pred_lt h
+    have h' := push as.pop (as.get ⟨as.size - 1, this⟩)
+    specialize h' (ind_push (motive := motive) empty push as.pop)
+    simp at h'
+    rw [Array.push_pop as this] at h'
+    exact h'
+termination_by _ => as.size
+
+end ind
