ArrowPoly/Poly.lean
@@ -3,19 +3,23 @@ import ArrowPoly.IntExtra
 
 attribute [local instance] Array.lexicographic
 
+local instance : LT (Array Int) := ltOfOrd
+
 structure Monomial where
   exponents : Array Int
   coeff : Int
-  (coeff_nonzero : coeff ≠ 0 := by simp [*])
-  (exp_norm : exponents.back? ≠ some 0 := by simp [*])
-  deriving Repr, Ord
+  coeff_nonzero : coeff ≠ 0 := by simp [*]
+  exp_norm : exponents.back? ≠ some 0 := by simp [*]
+  deriving Repr
 
--- Should have proof that the Monomial.exponents are in strictly increasing order
-def Poly := Array Monomial deriving Repr
+structure Poly where
+  terms : Array Monomial
+  incr : (terms.map Monomial.exponents).strictIncreasing
+  deriving Repr
 
-def Poly.mk (a : Array Monomial) : Poly := a
-
-def Poly.toArray (p : Poly) : Array Monomial := p
+def Poly.zero : Poly where
+  terms := #[]
+  incr := by intros i; cases i.isLt
 
 def Monomial.incl (n : Int) (hn : n ≠ 0 := by simp) : Monomial where
   coeff := n
@@ -33,30 +37,33 @@ def Monomial.scale (m : Monomial) (n : Int) (hn : n ≠ 0) : Monomial where
 
 def Monomial.mul (m₁ m₂ : Monomial) : Monomial where
   coeff := m₁.coeff * m₂.coeff
-  exponents := (Array.zipWith' m₁.exponents m₂.exponents (. + .)).dropZeros
+  exponents := (Array.zipWith' m₁.exponents m₂.exponents (. + .)).popZeros
   coeff_nonzero := by
     intro h
     cases Int.eq_zero_or_eq_zero_of_mul_eq_zero _ _ h
     apply m₁.coeff_nonzero; assumption
     apply m₂.coeff_nonzero; assumption
-  exp_norm := Array.back?_dropZeros _
+  exp_norm := Array.back?_popZeros _
 
 def Poly.add (p₁ p₂ : Poly) : Poly :=
-  let f (p : Poly) : Merge Monomial → Poly
-    | .left m₁ => p.push m₁ 
+  let f (p : Array Monomial) : Merge Monomial → Array Monomial
+    | .left m₁ => p.push m₁
     | .right m₂ => p.push m₂
     | .both m₁ m₂ =>
       if h : m₁.coeff + m₂.coeff = 0 then
         p
       else
         p.push <| {m₁ with coeff := m₁.coeff + m₂.coeff, coeff_nonzero := h}
-  Array.mergeBy Monomial.exponents f p₁ p₂
+  let p := Array.mergeBy Monomial.exponents f #[] p₁.terms p₂.terms
+  have : (p.map Monomial.exponents).strictIncreasing := by
+    sorry
+  ⟨p, this⟩
 
 instance : Add Poly where
   add := Poly.add
 
 def Poly.sub (p₁ p₂ : Poly) : Poly :=
-  let f p : Merge Monomial → Poly
+  let f (p : Array Monomial) : Merge Monomial → Array Monomial
     | .left m₁ => p.push m₁ 
     | .right m₂ => p.push {m₂ with coeff := -m₂.coeff, coeff_nonzero := by simp [m₂.coeff_nonzero]}
     | .both m₁ m₂ =>
@@ -64,16 +71,20 @@ def Poly.sub (p₁ p₂ : Poly) : Poly :=
         p
       else
         p.push <| {m₁ with coeff := m₁.coeff - m₂.coeff, coeff_nonzero := h}
-  Array.mergeBy Monomial.exponents f p₁ p₂
+  let p := Array.mergeBy Monomial.exponents f #[] p₁.terms p₂.terms
+  have : (p.map Monomial.exponents).strictIncreasing := by
+    sorry
+  ⟨p, this⟩
 
 instance : Sub Poly where
   sub := Poly.sub
 
-def Poly.mulScalar (p : Poly) (c : Int) (hc : c ≠ 0) : Poly :=
-  p.map (λ m => m.scale c hc)
+def Poly.mulScalar (p : Poly) (c : Int) (hc : c ≠ 0) : Poly where
+  terms := p.terms.map (λ m => m.scale c hc)
+  incr := sorry
 
 instance : HMul Int Poly Poly where
-  hMul c p := if h : c = 0 then #[] else p.mulScalar c h
+  hMul c p := if h : c = 0 then Poly.zero else p.mulScalar c h
 
 instance : Neg Poly where
   neg p := (-1 : Int) * p
@@ -82,29 +93,41 @@ def Poly.mulMonomial (p : Poly) (m : Monomial) : Poly :=
   if m.exponents.size = 0 then
     m.coeff * p
   else
-    p.map m.mul
+    { terms := p.terms.map m.mul,
+      incr := sorry }
 
 def Poly.mul (p₁ p₂ : Poly) : Poly := Id.run do
-  let mut q : Poly := #[]
-  for m₂ in p₂.toArray do
+  let mut q : Poly := Poly.zero
+  for m₂ in p₂.terms do
     q := q + p₁.mulMonomial m₂
   return q
 
 instance : Mul Poly where
   mul := Poly.mul
 
+instance : Coe Monomial Poly where
+  coe m :=
+    { terms := #[m],
+      incr := by
+        intros i j hij
+        cases i with | mk i hi =>
+        cases j with | mk j hj =>
+        have hi : i < 1 := hi
+        have hj : j < 1 := hj
+        simp at hi hj
+        cases hi
+        cases hj
+        cases hij }
+
 instance : Pow Poly Nat where
   pow :=
     let rec aux : Poly → Nat → Poly
-      | p, 0 => #[Monomial.incl 1]
+      | p, 0 => Monomial.incl 1
       | p, (n+1) => aux p n * p
     aux
 
-instance : Coe Monomial Poly where
-  coe m := #[m]
-
 instance : Coe Int Poly where
-  coe n := if h : n = 0 then #[] else #[Monomial.incl n h]
+  coe n := if h : n = 0 then Poly.zero else Monomial.incl n h
 
 instance : OfNat Poly n where
   ofNat := (n : Int)
@@ -117,14 +140,23 @@ def b : Poly := Monomial.mk #[3] 3
 
 def Poly.A (exp : Int := 1) : Poly :=
   if he : exp = 0 then Monomial.incl 1
-  else #[{coeff := 1,
-          exponents := #[exp],
-          exp_norm := by { show some exp ≠ some 0; simp [he] }}]
+  else { coeff := 1, exponents := #[exp],
+         exp_norm := by { show some exp ≠ some 0; simp [he] } : Monomial }
 
 def Poly.K (i : Nat) (exp : Nat := 1) : Poly :=
   if he : exp = 0 then Monomial.incl 1
-  else #[{coeff := 1, exponents := (Array.mkArray (i+1) 0).push exp}]
+  else {coeff := 1, exponents := (Array.mkArray (i+1) 0).push exp : Monomial }
 
 #eval Poly.A (-1) * (Poly.K 1 + Poly.K 2) * (Poly.K 1 + Poly.K 2) * Poly.A
 
 #eval (1 + Poly.A) ^ 6
+
+#eval (1 : Poly) + 1
+#eval 1 + Poly.A - 1
+#eval Poly.A + 1 - 1
+
+deriving instance Repr for Ordering
+
+#eval compare #[1] #[1,0]
+#eval Poly.A
+#eval Poly.A + Poly.A
