ArrowPoly/ListExtra.lean
@@ -1,0 +1,74 @@
+import ArrowPoly.NatExtra
+
+theorem List.concat_cons (x : α) (xs : List α) (y : α) :
+  (x :: xs).concat y = x :: xs.concat y := rfl
+
+@[simp]
+theorem List.get_concat_cons (x y : α) (xs : List α) (i : Fin (xs.concat y).length) :
+  ((x :: xs).concat y).get i.succ = (xs.concat y).get i := rfl
+
+@[simp]
+theorem List.get_concat_last (xs : List α) (y : α) (h : xs.length < (xs.concat y).length) :
+  (xs.concat y).get ⟨xs.length, h⟩ = y :=
+by
+  induction xs with
+  | nil => rfl
+  | cons x xs ih =>
+    have : length xs < length (concat xs y) := by
+      simp
+      apply Nat.lt_succ_self
+    have := List.get_concat_cons x y xs ⟨xs.length, this⟩
+    rw [ih] at this
+    exact this
+
+theorem List.get_concat (xs : List α) (a : α) (i : Nat) (h : i < xs.length) :
+  (xs.concat a).get ⟨i, by { simp; apply Nat.lt.step h }⟩ = xs.get ⟨i, h⟩ :=
+by
+  induction xs generalizing i with
+  | nil => cases h
+  | cons x xs ih =>
+    cases i with
+    | zero => simp [List.get]
+    | succ i =>
+      simp [List.get]
+      simp at h
+      exact ih i h
+
+theorem List.concat_dropLast_eq (xs : List α) (h : xs ≠ []) :
+  xs.dropLast.concat (xs.getLast h) = xs :=
+by
+  induction xs with
+  | nil => simp at h
+  | cons x xs ih =>
+    cases xs with
+    | nil => rfl
+    | cons x' xs =>
+      simp [dropLast, concat_cons, getLast]
+      apply ih
+
+theorem List.length_eq_zero_iff : {xs : List α} → xs.length = 0 ↔ xs = nil
+| [] => by simp
+| x :: xs => by simp
+
+theorem List.concat_ind {motive : List α → Prop}
+  (nil : motive [])
+  (concat : (xs : List α) → (x : α) → motive xs → motive (xs.concat x))
+  (xs : List α) : motive xs :=
+by
+  generalize h : xs.length = n
+  induction n generalizing xs with
+  | zero =>
+    simp [List.length_eq_zero_iff] at h
+    cases h
+    assumption
+  | succ n ih =>
+    cases xs with
+    | nil => simp at h
+    | cons x xs =>
+      simp at h
+      cases h
+      have := List.concat_dropLast_eq (x :: xs) (by simp)
+      rw [← this]
+      apply concat
+      apply ih
+      simp
