ArrowPoly/LogicExtra.lean
@@ -1,0 +1,11 @@
+theorem not_or (p q) : ¬ (p ∨ q) ↔ ¬ p ∧ ¬ q :=
+⟨fun H => ⟨mt Or.inl H, mt Or.inr H⟩, fun ⟨hp, hq⟩ pq => pq.elim hp hq⟩
+
+@[simp]
+theorem not_not (p : Prop) : ¬¬p ↔ p := by
+  cases Classical.em p with
+  | inl h => simp [h]
+  | inr h => simp [h]
+
+theorem Function.mt {p q : Prop} (f : p → q) : ¬ q → ¬ p :=
+λ hnq p => (hnq (f p)).elim
