ArrowPoly/NatExtra.lean
@@ -1,0 +1,26 @@
+@[simp] theorem Nat.succ_lt_succ_iff (m n : Nat) : m.succ < n.succ ↔ m < n :=
+⟨Nat.lt_of_succ_lt_succ, Nat.succ_lt_succ⟩
+
+theorem Nat.pred_le_self_of_ne_zero (m : Nat) (h : m ≠ 0) : m - 1 < m :=
+by cases m with
+   | zero => exact (h rfl).elim
+   | succ m => apply Nat.le_refl
+
+theorem Nat.pred_le_self_iff_ne_zero (m : Nat) : m - 1 < m ↔ m ≠ 0 where
+  mpr := Nat.pred_le_self_of_ne_zero m
+  mp := by
+    intro h
+    cases m with
+    | zero => cases h
+    | succ m => simp
+
+theorem Nat.eq_of_not_lt_and_lt_succ {m n : Nat} (hn : ¬ m < n) (h : m < n + 1) :
+  m = n :=
+Nat.le_antisymm (Nat.le_of_lt_succ h) (Nat.ge_of_not_lt hn)
+
+@[simp] theorem Nat.lt_one_iff_eq_zero : {m : Nat} → m < 1 ↔ m = 0
+| 0 => by simp
+| m+1 => by
+  simp [Nat.not_lt_zero]
+  intro h
+  cases h
